Squash commit of extension of world for sealing
WIP third world component for sealing

WIP third world component for sealing: `gmap OType (gset Word)` instead of `gset OType`

Fix context def world + define sealing_map (interp of world) + WIP logrel and FTLR

Fix compilation

Fix FLTR Seal and Unseal

Fix switcher specs

WIP fix examples

Fix lemma `sealing_map_def_alloc`

Fix deep immutability example

WIP fix examples

Fix counter example

Fix deep locality example

Fix LSE example

Fix CMDC example

Fix allocation of compartment + make ot_switcher_prop stable by borrowing + change seal_std_update to extend only

Fix DLE example

Fix SO example

WIP fix VAE example

Fix DROE example

Minor simplification DLE adequacy

Fix CMDC example

Fix LSE example

Fix VAE example

Rebase: fix compilation world_ghost_theory.v

Rebase: minor fixes

Rebase: finish to fix the rebase

Make `sealing_map_def` and related lemmas Local

Normalise the set of words in definition `sealing_map` to avoid having duplicates modulo locality

theories/opsem/machine_word.v
@@ -254,6 +254,19 @@ Definition load_word_perm (pload p : Perm) :=
                          )
   end.
 
+Definition force_global_sb (sb : Sealable) :=
+  match sb with
+  | SSealRange sp _ b e a => SSealRange sp Global b e a
+  | SCap p _ b e a => SCap p Global b e a
+  end.
+
+Definition force_global (w : Word) :=
+  match w with
+  | WSealable sb => WSealable (force_global_sb sb)
+  | WSentry p _ b e a => WSentry p Global b e a
+  | WSealed ot sb => WSealed ot (force_global_sb sb)
+  | _ => w
+  end.
 
 
 Definition PermFlowsToCap (p: Perm) (w: Word) : bool :=
@@ -625,6 +638,18 @@ Proof.
   destruct w as [| [|] | |]; cbn in *; simplify_eq; auto.
   destruct sb; cbn in *; auto; destruct g; cbn in *; auto.
 Qed.
+
+Lemma borrow_sb_idempotent (sb : Sealable) :
+  (borrow_sb (borrow_sb sb)) = (borrow_sb sb).
+Proof. by destruct sb; cbn. Qed.
+
+Lemma force_global_borrow_sb (sb : Sealable) :
+  (force_global_sb (borrow_sb sb)) = (force_global_sb sb).
+Proof. by destruct sb; cbn. Qed.
+
+Lemma force_global_borrow (w : Word) :
+  (force_global (borrow w)) = (force_global w).
+Proof. destruct w ; cbn; auto; rewrite force_global_borrow_sb; done.  Qed.
 
 Ltac entry_point_inj :=
   try ( apply seal_capability_inj; auto )
