theories/case_studies/stack_object/stack_object_spec_resources.v
@@ -56,7 +56,7 @@ Section Stack_Object_Region_Resources.
     {Σ : gFunctors}
     {ceriseg : ceriseG Σ} {sealsg : sealStoreG Σ}
     {Cname : CmptNameG} {CNames : gset CmptName}
-    {stsg : STSG Addr region_type Σ}
+    {stsg : STSG Addr region_type OType Word Σ}
     {relg : relGS Σ} {cstackg : CSTACKG Σ}
     `{MP : MachineParameters}.
 
