theories/model/model_interp_stack.v
@@ -9,7 +9,7 @@ Section WorldInterpStack.
     {Σ:gFunctors}
     {ceriseg:ceriseG Σ} {sealsg: sealStoreG Σ}
     {Cname : CmptNameG}
-    {stsg : STSG Addr region_type Σ} {cstackg : CSTACKG Σ} {relg : relGS Σ}
+    {stsg : STSG Addr region_type OType Word Σ} {cstackg : CSTACKG Σ} {relg : relGS Σ}
     `{MP: MachineParameters}
   .
 
