theories/switcher/switcher_spec_return_blocks.v
@@ -8,7 +8,7 @@ Section Switcher_Return_Blocks.
     {Σ:gFunctors}
     {ceriseg:ceriseG Σ} {sealsg: sealStoreG Σ}
     {Cname : CmptNameG}
-    {stsg : STSG Addr region_type Σ}
+    {stsg : STSG Addr region_type OType Word Σ}
     {cstackg : CSTACKG Σ} {relg : relGS Σ}
     `{MP: MachineParameters}
     {swlayout : switcherLayout} {swlayoutwf : switcherLayoutWf}
